Versions/Bookmarker.i.dfy
@@ -44,67 +44,6 @@ module Bookmarker {
 
   /// Invariant definition
 
-  predicate IsPath(
-      k: SM.Constants,
-      s: SM.Variables,
-      uiops: seq<SM.UIOp>,
-      s': SM.Variables,
-      states: seq<SM.Variables>)
-  {
-    && |states| == |uiops| + 1
-    && states[0] == s
-    && states[|states|-1] == s'
-    && forall i | 0 <= i < |uiops| ::
-        SM.Next(k, states[i], states[i+1], uiops[i])
-  }
-
-  predicate path(
-      k: SM.Constants,
-      s: SM.Variables,
-      jes: seq<JournalEntry>,
-      s': SM.Variables)
-  {
-    exists states, uiops ::
-        && jes == JournalEntriesForUIOps(uiops)
-        && IsPath(k, s, uiops, s', states)
-  }
-
-  predicate IsSuffix<T>(s: seq<T>, t: seq<T>)
-  {
-    && |t| <= |s|
-    && s[|s| - |t| ..] == t
-  }
-
-  // Sequence subtraction s-t
-  // Only makes sense when t is a suffix of s.
-  // Result is that s-t+t == s for the usual notion
-  // of sequence addition.
-  function {:opaque} SeqSub<T>(s: seq<T>, t: seq<T>) : seq<T>
-  requires IsSuffix(s, t)
-  ensures SeqSub(s, t) + t == s
-  {
-    s[.. |s| - |t|]
-  }
-
-  lemma SeqSubAdd<T>(a: seq<T>, b: seq<T>, c: seq<T>, d: seq<T>)
-  requires IsSuffix(a, b)
-  requires IsSuffix(b + c, d)
-  ensures SeqSub(a, b) + SeqSub(b + c, d)
-      == SeqSub(a + c, d)
-  {
-    reveal_SeqSub();
-  }
-
-  predicate advances(k: SM.Constants,
-      s: SM.Variables,
-      jes: seq<JournalEntry>, 
-      s': SM.Variables,
-      jes2: seq<JournalEntry>)
-  {
-    && IsSuffix(jes, jes2)
-    && path(k, s, SeqSub(jes, jes2), s')
-  }
-
   function s1(s: Variables) : SM.Variables
   requires s.jc.persistentLoc in s.tsm.disk
   {
@@ -135,8 +74,8 @@ module Bookmarker {
       && s.tsm.frozenLoc == s.jc.frozenLoc
     )
     && (s.tsm.persistentLoc.Some? ==>
-      || s.tsm.persistentLoc.value == s.jc.persistentLoc
-      || s.tsm.frozenLoc == Some(s.jc.persistentLoc)
+      || s.jc.persistentLoc == s.tsm.persistentLoc.value
+      || Some(s.jc.persistentLoc) == s.jc.frozenLoc
     )
     && (s.tsm.frozenLoc.Some? ==>
       && s.tsm.frozenLoc.value in s.tsm.disk
@@ -156,66 +95,8 @@ module Bookmarker {
     && SM.Inv(k.tsm.k, s2(s))
     && SM.Inv(k.tsm.k, s3(s))
 
-    && advances(k.tsm.k, s1(s), s.jc.j_gamma, s2(s), s.jc.j2)
-    && advances(k.tsm.k, s2(s), s.jc.j2 + s.jc.j_delta, s3(s), s.jc.j3)
-  }
-
-  lemma path_empty(k: SM.Constants, s: SM.Variables)
-  ensures path(k, s, [], s)
-  {
-    var states := [s];
-    var uiops := [];
-    assert [] == JournalEntriesForUIOps(uiops);
-    assert IsPath(k, s, uiops, s, states);
-  }
-
-  lemma paths_compose(k: SM.Constants, s1: SM.Variables, jes1: seq<JournalEntry>, s2: SM.Variables, jes2: seq<JournalEntry>, s3: SM.Variables)
-  requires path(k, s1, jes1, s2)
-  requires path(k, s2, jes2, s3)
-  ensures path(k, s1, jes1 + jes2, s3)
-  {
-    var states1, uiops1 :|
-        && jes1 == JournalEntriesForUIOps(uiops1)
-        && IsPath(k, s1, uiops1, s2, states1);
-    var states2, uiops2 :|
-        && jes2 == JournalEntriesForUIOps(uiops2)
-        && IsPath(k, s2, uiops2, s3, states2);
-
-    var states := states1 + states2[1..];
-    var uiops := uiops1 + uiops2;
-
-    JournalEntriesForUIOpsAdditive(uiops1, uiops2);
-    assert jes1 + jes2 == JournalEntriesForUIOps(uiops);
-
-    forall i | 0 <= i < |uiops|
-    ensures SM.Next(k, states[i], states[i+1], uiops[i]);
-    {
-      if i < |uiops1| {
-        assert states[i] == states1[i];
-        assert states[i+1] == states1[i+1];
-        assert uiops[i] == uiops1[i];
-        assert SM.Next(k, states1[i], states1[i+1], uiops1[i]);
-      } else {
-        assert states[i] == states2[i - |uiops1|];
-        assert states[i+1] == states2[i - |uiops1| + 1];
-        assert uiops[i] == uiops2[i - |uiops1|];
-        assert SM.Next(k, states2[i - |uiops1|],
-            states2[i - |uiops1| + 1], uiops2[i - |uiops1|]);
-      }
-    }
-    assert IsPath(k, s1, uiops, s3, states);
-  }
-
-  lemma path_append(k: SM.Constants, s1: SM.Variables, jes: seq<JournalEntry>, s2: SM.Variables, uiop: SM.UIOp, s3: SM.Variables)
-  requires path(k, s1, jes, s2)
-  requires SM.Next(k, s2, s3, uiop)
-  ensures path(k, s1, jes + JournalEntriesForUIOp(uiop), s3)
-  {
-    var jes2 := JournalEntriesForUIOp(uiop);
-    assert jes2 == JournalEntriesForUIOps([uiop]);
-    assert IsPath(k, s2, [uiop], s3, [s2, s3]);
-    assert path(k, s2, jes2, s3);
-    paths_compose(k, s1, jes, s2, jes2, s3);
+    //&& advances(k.tsm.k, s1(s), s.jc.j_gamma, s2(s), s.jc.j2)
+    //&& advances(k.tsm.k, s2(s), s.jc.j2 + s.jc.j_delta, s3(s), s.jc.j3)
   }
 
   lemma InitImpliesInv(k: Constants, s: Variables, s': Variables)
@@ -223,7 +104,6 @@ module Bookmarker {
   ensures Inv(k, s)
   {
     SM.InitImpliesInv(k.tsm.k, s1(s));
-    path_empty(k.tsm.k, s1(s));
   }
 
   lemma Move3PreservesInv(k: Constants, s: Variables, s': Variables, vop: VOp, uiop: UI.Op)
@@ -233,24 +113,6 @@ module Bookmarker {
   requires Inv(k, s)
   ensures Inv(k, s')
   {
-    SM.NextPreservesInv(k.tsm.k, s3(s), s3(s'), vop.uiop);
-    var new_je := JournalEntriesForUIOp(vop.uiop);
-    path_append(k.tsm.k, s2(s), s.jc.j2 + s.jc.j_delta, s3(s), vop.uiop, s3(s'));
-
-    assert s1(s) == s1(s');
-    assert s2(s) == s2(s');
-
-    assert s.jc.j3 == [];
-    assert SeqSub(s.jc.j2 + s.jc.j_delta, s.jc.j3)
-        == s.jc.j2 + s.jc.j_delta;
-    assert SeqSub(s.jc.j2 + s.jc.j_delta + JournalEntriesForUIOp(vop.uiop), s.jc.j3)
-        == s.jc.j2 + s.jc.j_delta + JournalEntriesForUIOp(vop.uiop);
-
-    assert path(k.tsm.k, s2(s), s.jc.j2 + s.jc.j_delta + new_je, s3(s'));
-    assert path(k.tsm.k, s2(s'), SeqSub(s'.jc.j2 + s'.jc.j_delta, s'.jc.j3), s3(s'));
-    assert advances(k.tsm.k, s2(s'), s'.jc.j2 + s'.jc.j_delta, s3(s'), s'.jc.j3);
-
-    assert Inv(k, s');
   }
 
   lemma ReplayPreservesInv(k: Constants, s: Variables, s': Variables, vop: VOp, uiop: UI.Op)
@@ -260,11 +122,6 @@ module Bookmarker {
   requires Inv(k, s)
   ensures Inv(k, s')
   {
-    SM.NextPreservesInv(k.tsm.k, s3(s), s3(s'), vop.uiop);
-    path_append(k.tsm.k, s2(s), SeqSub(s.jc.j2 + s.jc.j_delta, s.jc.j3), s3(s), vop.uiop, s3(s'));
-    assert SeqSub(s.jc.j2 + s.jc.j_delta, s.jc.j3) + JournalEntriesForUIOp(vop.uiop)
-        == SeqSub(s.jc.j2 + s.jc.j_delta, s'.jc.j3);
-    assert Inv(k, s');
   }
 
   lemma AdvancePreservesInv(k: Constants, s: Variables, s': Variables, vop: VOp, uiop: UI.Op)
@@ -286,17 +143,16 @@ module Bookmarker {
   requires Inv(k, s)
   ensures Inv(k, s')
   {
-    path_empty(k.tsm.k, s2(s));
-    path_empty(k.tsm.k, s3(s));
-    paths_compose(k.tsm.k, s1(s),
-        SeqSub(s.jc.j_gamma, s.jc.j2),
-        s2(s),
-        SeqSub(s.jc.j2 + s.jc.j_delta, s.jc.j3),
-        s3(s));
-    SeqSubAdd(s.jc.j_gamma, s.jc.j2, s.jc.j_delta, s.jc.j3);
-    assert SeqSub(s.jc.j_gamma, s.jc.j2) + SeqSub(s.jc.j2 + s.jc.j_delta, s.jc.j3)
-        == SeqSub(s.jc.j_gamma + s.jc.j_delta, s.jc.j3);
-    assert advances(k.tsm.k, s1(s), s.jc.j_gamma + s.jc.j_delta, s3(s), s.jc.j3);
+    assert JournalChain.Move2to3(k.jc, s.jc, s'.jc, vop);
+    assert TriStateMap.Freeze(k.tsm, s.tsm, s'.tsm, vop);
+
+    /*assert s.jc.frozenLoc != Some(s.jc.persistentLoc);
+    if s.tsm.persistentLoc.Some? {
+      if s.tsm.frozenLoc == Some(s.jc.persistentLoc) {
+        assert s.tsm.frozenLoc != s.jc.frozenLoc;
+      }
+      assert s.jc.persistentLoc == s.tsm.persistentLoc.value;
+    }*/
   }
 
   lemma NextStepPreservesInv(k: Constants, s: Variables, s': Variables, vop: VOp, uiop: UI.Op)
@@ -313,7 +169,6 @@ module Bookmarker {
         AdvancePreservesInv(k, s, s', vop, uiop);
       }
       case CrashOp => {
-        path_empty(k.tsm.k, s1(s));
         assert s1(s) == s1(s') == s2(s') == s3(s');
         assert JournalChain.Crash(k.jc, s.jc, s'.jc, vop);
         assert TriStateMap.Crash(k.tsm, s.tsm, s'.tsm, vop);
